Move stuff from the MoreGeneral file

src/MoreGeneral.v
@@ -1,3 +1,10 @@
+(** * The more general relations
+      This file contains the defintions of more general schemes [more_general] and more 
+      contexts [more_general_ctx].
+      Several lemmas about the two relations are necessary for the let case in the
+      completeness proof of algorithm W.
+    *)
+
 Set Implicit Arguments.
 
 Require Import Omega.
@@ -14,7 +21,9 @@ Require Import NewTypeVariable.
 Require Import SimpleTypes.
 Require Import Subst.
 Require Import MyLtacs.
-
+Require Import Nth_error_tools.
+Require Import Product_list.
+Require Import Prefix.
 Require Import LibTactics.
 
 Inductive more_general : schm -> schm -> Prop :=
@@ -24,65 +33,12 @@ Inductive more_general : schm -> schm -> Prop :=
 
 Hint Constructors more_general.
 
-Inductive more_general_ctx : ctx -> ctx -> Prop :=
-| more_general_ctx_nil : more_general_ctx nil nil
-| more_general_ctx_cons : forall (G1 G2 : ctx) (i : id) (sigma1 sigma2 : schm),
-    more_general_ctx G1 G2 -> more_general sigma1 sigma2 ->
-    more_general_ctx ((i, sigma1) :: G1) ((i, sigma2) :: G2).
+(** ** More general schemes lemmas *)
 
-Hint Constructors more_general_ctx.
-
-Fixpoint product_list (l1 : list id) (l2 : list ty) :=
-  match l1 with
-  | nil =>  Some nil
-  | st :: l'1 => match l2 with
-                | nil => None
-                | t :: l'2 => match product_list l'1 l'2 with
-                             | None => None
-                             | Some s => Some ((st, t) :: s)
-                             end
-                end
-  end.
-
-Fixpoint ty_from_id_list (l : list id) : list ty :=
-  match l with
-  | nil => nil
-  | x::l' => var x :: ty_from_id_list l'
-  end.
-
-Lemma ty_from_id_list_app : forall l1 l2 : list id,
-    ty_from_id_list (l1 ++ l2) = ty_from_id_list l1 ++ ty_from_id_list l2.
-Proof.
-  induction l1; crush.
-Qed.
-
-Hint Resolve ty_from_id_list_app.
-Hint Rewrite ty_from_id_list_app:RE.
-
-Fixpoint map_extend_subst_type (l : list ty) (s2 : substitution) :=
-  match l with
-  | nil => nil
-  | t::l' => apply_subst s2 t :: map_extend_subst_type l' s2
-  end.
-
-Lemma map_extend_app : forall (s : substitution) (l1 l2 : list ty),
-    map_extend_subst_type (l1 ++ l2) s = map_extend_subst_type l1 s ++ map_extend_subst_type l2 s.
-Proof.
-  induction l1; crush.
-Qed.
-
-Hint Resolve map_extend_app.
-Hint Rewrite map_extend_app:RE.
-
-Inductive is_prefixe_free2 : list id -> list id -> list id -> Prop :=
-|  prefixe_free2_intro : forall C l L : list id,
-    {l1 : list id | L = l ++ l1 /\ are_disjoints C l1} -> is_prefixe_free2 C l L.
-
-Hint Constructors is_prefixe_free2.
-
-Lemma more_general_in_list_FV_schm : forall sigma1 sigma2, more_general sigma1 sigma2 ->
-                                                      forall i, in_list_id i (FV_schm sigma1) = true ->
-                                                           in_list_id i (FV_schm sigma2) = true.
+Lemma more_general_in_list_FV_schm : forall sigma1 sigma2,
+    more_general sigma1 sigma2 ->
+    forall i, in_list_id i (FV_schm sigma1) = true ->
+         in_list_id i (FV_schm sigma2) = true.
 Proof.
   induction sigma1; eauto.
   - intros.
@@ -108,66 +64,6 @@ Proof.
     edestruct H1.
 Abort.
 
-Fixpoint find_instance (sigma : schm) (tau : ty) :=
-  match sigma with
-  | sc_con i => con i
-  | sc_var i => var i
-  | sc_gen st => tau
-  | sc_arrow sigma1 sigma2 => arrow (find_instance sigma1 tau) (find_instance sigma2 tau)
-  end.
-
-Fixpoint make_constant_inst_subst (n : id) (tau : ty)  :=
-  match n with
-  | O => nil 
-  | S p => tau :: make_constant_inst_subst p tau
-  end.
-Lemma nth_error_make_constant_inst_subst3 : forall (p n : id) (tau : ty),
-    S n <= p -> nth_error (make_constant_inst_subst p tau) n = Some tau.
-Proof.
-  induction p; crush.
-  destruct n; crush.
-  apply IHp.
-  auto with *.
-Qed.
-
-Hint Resolve nth_error_make_constant_inst_subst3.
-Hint Rewrite nth_error_make_constant_inst_subst3:RE.
-
-Lemma apply_subst_inst_make_constant_inst_subst : forall (sigma : schm) (tau : ty) (p : id),
-    max_gen_vars sigma <= p ->
-    apply_inst_subst (make_constant_inst_subst p tau) sigma = Some (find_instance sigma tau).
-Proof.
-  induction sigma; eauto.
-  unfold max_gen_vars.
-  unfold apply_inst_subst.
-  intros tau p le.
-  simpl in le.
-  crush.
-  intros tau p le.
-  simpl.
-  erewrite (IHsigma1 tau p); eauto.
-  erewrite (IHsigma2 tau p); eauto.
-  eauto with *.
-  simpl in le.
-  pose proof (PeanoNat.Nat.le_max_l (max_gen_vars sigma1) (max_gen_vars sigma2)).
-  auto with *.
-Qed.
-
-Hint Resolve apply_subst_inst_make_constant_inst_subst.
-Hint Resolve apply_subst_inst_make_constant_inst_subst:RE.
-
-Lemma find_some_instance_of_some_sigma : forall (sigma : schm) (tau : ty),
-    is_schm_instance (find_instance sigma tau) sigma.
-Proof.
-  intros.
-  unfold is_schm_instance.
-  exists (make_constant_inst_subst (max_gen_vars sigma) tau).
-  auto.
-Qed.
-
-Hint Resolve find_some_instance_of_some_sigma.
-Hint Rewrite find_some_instance_of_some_sigma:RE.
-
 Lemma sc_var_more_general_than_sigma : forall (sigma : schm) (st : id),
     more_general (sc_var st) sigma -> sigma = sc_var st.
 Proof.
@@ -188,144 +84,6 @@ Qed.
 Hint Resolve sc_var_more_general_than_sigma.
 Hint Rewrite sc_var_more_general_than_sigma:RE.
 
-Lemma var_is_not_instance_of_arrow : forall (sigma1 sigma2 : schm) (i : id),
-    ~ is_schm_instance (var i) (sc_arrow sigma1 sigma2).
-Proof.
-  intros. intro.
-  inverts* H.
-  apply exist_arrow_apply_inst_arrow2 in H0.
-  destruct H0 as [tau1 [tau2 H]].
-  destruct H.
-  destruct H0.
-  inverts* H1.
-Qed.
-
-Hint Resolve var_is_not_instance_of_arrow.
-
-Lemma con_is_not_instance_of_arrow : forall (sigma1 sigma2 : schm) (i : id),
-    ~ is_schm_instance (con i) (sc_arrow sigma1 sigma2).
-Proof.
-  intros. intro.
-  inverts* H.
-  apply exist_arrow_apply_inst_arrow2 in H0.
-  destruct H0 as [tau1 [tau2 H]].
-  destruct H.
-  destruct H0.
-  inverts* H1.
-Qed.
-
-Hint Resolve con_is_not_instance_of_arrow.
-
-Lemma arrow_sigma_more_general_than_arrow : forall sigma sigma1 sigma2 : schm,
-    (forall tau : ty, is_schm_instance tau sigma -> is_schm_instance tau (sc_arrow sigma1 sigma2)) ->
-    {sig_sig : schm * schm | sigma = sc_arrow (fst sig_sig) (snd sig_sig)}.
-Proof.
-  induction sigma. 
-  - cut (is_schm_instance (find_instance (sc_var i) (con i)) (sc_var i)); auto.
-    intros.
-    cut (is_schm_instance (find_instance (sc_var i) (con i)) (sc_arrow sigma1 sigma2)); auto.
-    intros.
-    simpl in *.
-    absurd (is_schm_instance (var i) (sc_arrow sigma1 sigma2)); auto.
-  - intros.
-    assert (is_schm_instance (con i) (sc_con i)).
-    exists (nil:inst_subst). reflexivity.
-    apply H in H0. 
-    apply con_is_not_instance_of_arrow in H0.
-    contradiction.
-  - intros.
-    cut (is_schm_instance (find_instance (sc_gen i) (con i)) (sc_gen i)); auto.
-    intros.
-    cut (is_schm_instance (find_instance (sc_gen i) (con i)) (sc_arrow sigma1 sigma2)); auto.
-    intros.
-    absurd (is_schm_instance (con i) (sc_arrow sigma1 sigma2)); auto.
-  - intros.
-    exists (sigma1, sigma2). reflexivity.
-Qed.
-
-Hint Resolve arrow_sigma_more_general_than_arrow.
-Hint Resolve arrow_sigma_more_general_than_arrow:RE.
-
-Lemma length_map : forall (s : substitution) (l : list ty),
-    length (map_extend_subst_type l s) = length l.
-Proof.
-  induction l; crush.
-Qed.
-
-Hint Resolve length_map.
-Hint Rewrite length_map:RE.
-
-Lemma length_app : forall (A : Set) (l1 l2 : list A), length (l1 ++ l2) = length l1 + length l2.
-Proof.
-  induction l1; crush.
-Qed.
- 
-Hint Resolve length_app.
-
-Lemma length_make_constant_inst_subst : forall (n : nat) (t : ty), length (make_constant_inst_subst n t) = n.
-  induction n; crush.
-Qed.
-
-Hint Resolve length_make_constant_inst_subst.
-
-Lemma apply_inst_subst_succeeds : forall (sigma : schm) (is_s : inst_subst),
-    max_gen_vars sigma <= length is_s -> exists tau, apply_inst_subst is_s sigma = Some tau.
-Proof.
-  induction sigma; crush.
-  cases (nth_error is_s i).
-  exists t. reflexivity.
-  apply nth_error_None in Eq.
-  omega.
-  edestruct IHsigma1; eauto.
-  apply Nat.max_lub_l in H.
-  apply H.
-  edestruct IHsigma2; eauto.
-  apply Nat.max_lub_r in H.
-  apply H.
-  rewrite H0.
-  rewrite H1.
-  exists (arrow x x0). reflexivity.
-Qed.
-
-Hint Resolve apply_inst_subst_succeeds.
-
-Lemma apply_inst_subst_ge_app : forall (sigma : schm) (is_s l : inst_subst),
-    max_gen_vars sigma <= length is_s -> apply_inst_subst (is_s ++ l) sigma = apply_inst_subst is_s sigma.
-Proof.
-  induction sigma; crush.
-  cases (nth_error (is_s ++ l) i).
-  erewrite <- nth_error_app1; eauto.
-  rewrite Eq. reflexivity.
-  erewrite <- nth_error_app1; eauto.
-  rewrite Eq. reflexivity.
-  erewrite IHsigma1; eauto.
-  erewrite IHsigma2; eauto.
-  apply Nat.max_lub_r in H.
-  apply H.
-  apply Nat.max_lub_l in H.
-  apply H.
-Qed.
-
-Hint Resolve apply_inst_subst_ge_app.
-
-Lemma is_instance_le_max : forall (sigma : schm) (tau : ty) (is_s : inst_subst),
-    apply_inst_subst is_s sigma = Some tau -> max_gen_vars sigma <= length is_s.
-Proof.
-  induction sigma; crush.
-  cases (nth_error is_s i).
-  inverts* H.
-  assert (nth_error is_s i <> None). { intro. rewrite Eq in H. inversion H. }
-  apply nth_error_Some in H. omega.                                   
-  inversion H.
-  cases (apply_inst_subst is_s sigma1).
-  cases (apply_inst_subst is_s sigma2).
-  apply Nat.max_lub_iff; eauto.
-  inversion H.
-  inversion H.
-Qed.
-
-Hint Resolve is_instance_le_max.
-
 Lemma more_general_arrow_inversion1 : forall sigma1 sigma2 sigma1' sigma2' : schm,
     more_general (sc_arrow sigma1 sigma2) (sc_arrow sigma1' sigma2') ->
     more_general sigma1 sigma1'.
@@ -336,7 +94,7 @@ Proof.
   intros.
   inverts* H.
   destruct (apply_inst_subst_succeeds sigma2' (x ++ make_constant_inst_subst (max_gen_vars sigma2') (con 0))).
-  rewrite length_app.
+  rewrite app_length.
   rewrite length_make_constant_inst_subst.
   auto with *.
   cut (is_schm_instance (arrow tau x0) (sc_arrow sigma1 sigma2)).
@@ -368,7 +126,7 @@ Proof.
   intros.
   inverts* H.
   destruct (apply_inst_subst_succeeds sigma1' (x ++ make_constant_inst_subst (max_gen_vars sigma1') (con 0))).
-  rewrite length_app.
+  rewrite app_length.
   rewrite length_make_constant_inst_subst.
   auto with *.
   cut (is_schm_instance (arrow x0 tau) (sc_arrow sigma1 sigma2)).
@@ -393,8 +151,9 @@ Qed.
 
 Hint Resolve more_general_arrow_inversion2.
 
-Lemma FV_more_general : forall sigma1 sigma2 : schm, more_general sigma1 sigma2 ->
-                                              is_sublist_id (FV_schm sigma1) (FV_schm sigma2).
+Lemma FV_more_general : forall sigma1 sigma2 : schm,
+    more_general sigma1 sigma2 ->
+    is_sublist_id (FV_schm sigma1) (FV_schm sigma2).
 Proof.
   induction sigma1; crush.
   apply sc_var_more_general_than_sigma in H.
@@ -408,9 +167,21 @@ Proof.
 Qed.
 
 Hint Resolve FV_more_general.
+
+(** ** More general contexts lemmas *)
+
+Inductive more_general_ctx : ctx -> ctx -> Prop :=
+| more_general_ctx_nil : more_general_ctx nil nil
+| more_general_ctx_cons : forall (G1 G2 : ctx) (i : id) (sigma1 sigma2 : schm),
+    more_general_ctx G1 G2 -> more_general sigma1 sigma2 ->
+    more_general_ctx ((i, sigma1) :: G1) ((i, sigma2) :: G2).
+
+Hint Constructors more_general_ctx.
+
  
-Lemma FV_more_general_ctx : forall G1 G2 : ctx, more_general_ctx G1 G2 ->
-                                           Sublist.is_sublist_id (FV_ctx G1) (FV_ctx G2).
+Lemma FV_more_general_ctx : forall G1 G2 : ctx,
+    more_general_ctx G1 G2 ->
+    Sublist.is_sublist_id (FV_ctx G1) (FV_ctx G2).
 Proof.
   intros.
   induction H.
@@ -426,219 +197,10 @@ Qed.
 
 Hint Resolve FV_more_general_ctx.
 
-Lemma nth_error_app : forall (l l1 : list ty) (n : id), n < length l -> nth_error (l ++ l1) n = nth_error l n.
-Proof.
-  induction l; crush.
-  induction n; crush.
-  erewrite <- IHl; crush.
-Qed.
-
-Hint Resolve nth_error_app.
-Hint Rewrite nth_error_app:RE.
-
-Lemma domain_product : forall (l : list id) (is_s : inst_subst) (phi : substitution),
-    product_list l is_s = Some phi -> dom phi = l.
-Proof.
-  induction l. crush.
-  destruct is_s. crush.
-  intros. 
-  simpl in *.
-  cases (product_list l is_s).
-  inverts* H.
-  simpl.
-  erewrite IHl; eauto.
-  inverts* H.
-Qed.  
-
-Lemma index_list_id_nil : forall st, index_list_id st nil = None.
-Proof.
-  induction st; crush.
-Qed.
-
-Hint Resolve index_list_id_nil.
-Hint Rewrite index_list_id_nil:RE.
-
-Lemma index_aux1 : forall st l k n, index_list_id_aux (S n) st l = Some k -> index_list_id_aux n st l = Some (Nat.pred k).
-Proof.
-  induction l. crush.
-  intros.
-  simpl in *.
-  destruct (eq_id_dec a st).
-  subst.
-  inversion H. subst. reflexivity.
-  apply IHl in H. auto.
-Qed.
-
-Hint Resolve index_aux1.
-
-Lemma index_aux2 : forall st l k n, index_list_id_aux n st l = Some k -> index_list_id_aux (S n) st l = Some (S k).
-Proof.
-  induction l; crush.
-Qed.
-
-Hint Resolve index_aux2.
-
-Lemma index_aux_false : forall l n m i, m < n -> index_list_id_aux n i l = Some m -> False.
-Proof.
-  induction l; crush.
-  Unshelve.
-  auto.
-  auto.
-Qed.
-Hint Resolve index_aux_false.
-
-Lemma image_by_product2 : forall (l : list id) (is_s : inst_subst) (st : id) 
-                            (n0 : id) (phi : substitution) (tau : ty),
-    index_list_id st l = Some n0 ->
-    product_list l is_s = Some phi ->
-    nth_error is_s n0 = Some tau -> apply_subst phi (var st) = tau.
-Proof.
-  induction l; unfold index_list_id. crush.
-  intros.
-  simpl in *.
-  destruct (eq_id_dec a st).
-  inverts* H.
-  destruct is_s.
-  inversion H0.
-  subst.
-  simpl in H1. inverts* H1.
-  cases (product_list l is_s).
-  inverts* H0.
-  crush.
-  inversion H0.
-  destruct is_s.
-  inversion H0.
-  cases (product_list l is_s).
-  inverts* H0.
-  crush.
-  eapply IHl.
-  apply index_aux1 in H.
-  unfold index_list_id. apply H.
-  apply Eq.
-  destruct n0. simpl in *.
-  inverts* H1. destruct is_s.
-  assert (False). { eapply index_aux_false with (n := 1) (m := 0); eauto. } contradiction.
-  assert (False). { eapply index_aux_false with (n := 1) (m := 0); eauto. } contradiction.
-  simpl. eauto.
-  inversion H0.
-Qed.
-
-Hint Resolve image_by_product2.
-
-Lemma index_lt : forall (l : list id) (st : id) (k : id),
-    index_list_id st l = Some k -> k < length l.
-Proof.
-  induction l. unfold index_list_id in *. crush.
-  unfold index_list_id in *.
-  intros.
-  simpl in H.
-  destruct (eq_id_dec a st).
-  inversion H. subst.
-  simpl. auto with *.
-  apply index_aux1 in H.
-  apply IHl in H.
-  simpl. omega.
-Qed.
-
-Hint Resolve index_lt.
-
-Lemma index_list_none_any_k : forall l i k k', index_list_id_aux k i l = None -> index_list_id_aux k' i l = None.
-Proof.
-  induction l; crush.
-Qed.
-
-Hint Resolve index_list_none_any_k.
-
-Lemma index_list_id_cons : forall (l : list id) (i : id),
-    index_list_id i l = None -> index_list_id i (l ++ i::nil) = Some (length l).
-Proof.
-  induction l; unfold index_list_id in *; crush.
-Qed.
-
-Hint Resolve index_list_id_cons.
-
-Lemma index_list_id_aux_app : forall (l1 l2 : list id) (n : id) (i : id) k,
- index_list_id_aux k i l1 = Some n -> index_list_id_aux k i (l1 ++ l2) = Some n.
-Proof.
-  induction l1; unfold index_list_id in *; crush.
-Qed.
-
-Hint Resolve index_list_id_aux_app.
-
-Lemma index_list_id_app : forall (l1 l2 : list id) (n : id) (i : id),
- index_list_id i l1 = Some n -> index_list_id i (l1 ++ l2) = Some n.
-Proof.
-  induction l1; unfold index_list_id in *; crush.
-Qed.
-
-Hint Resolve index_list_id_app.
-
-Lemma Snd_gen_aux_with_app3 : forall (G : ctx) (tau : ty) (l : list id),
-    exists l', snd (gen_ty_aux tau G l) = l ++ l' /\ are_disjoints (FV_ctx G) l'.
-Proof.
-  induction tau.
-  - intro. simpl.
-    cases (in_list_id i (FV_ctx G)).
-    exists (nil : list id).
-    crush.
-    cases (index_list_id i l).
-    exists (nil : list id).
-    crush.
-    exists (i::nil : list id).
-    crush.
-  - crush.
-    exists (nil : list id).
-    crush.
-  - intros.
-    rewrite snd_gen_ty_aux_arrow_rewrite.
-    edestruct IHtau1.
-    destruct H.
-    rewrite H.
-    edestruct IHtau2.
-    destruct H1.
-    rewrite H1.
-    exists (x ++ x0).
-    split.
-    rewrite app_assoc. reflexivity.
-    eauto.
-Qed.
-
-Hint Resolve Snd_gen_aux_with_app3.
-
-Lemma disjoint_Snd_gen_aux : forall (G : ctx) (l : list id) (tau : ty),
-    are_disjoints (FV_ctx G) l -> are_disjoints (FV_ctx G) (snd (gen_ty_aux tau G l)).
-Proof.
-  intros.
-  destruct (Snd_gen_aux_with_app3 G tau l).
-  destruct H0. rewrite H0.
-  eauto.
-Qed.
-
-Hint Resolve disjoint_Snd_gen_aux.
-
-Lemma is_prefixe2_gen_aux : forall (l L : list id) (tau : ty) (G : ctx),
-    is_prefixe_free2 (FV_ctx G) (snd (gen_ty_aux tau G l)) L ->
-    is_prefixe_free2 (FV_ctx G) l L.
-Proof.
-  intros.
-  destruct (Snd_gen_aux_with_app3 G tau l).
-  destruct H0.
-  inverts* H.
-  destruct H2.
-  destruct a.
-  econstructor.
-  exists (x ++ x0).
-  split.
-  rewrite app_assoc.
-  rewrite <- H0.
-  rewrite H. reflexivity.
-  eauto.
-Qed.
-
-Hint Resolve is_prefixe2_gen_aux.
-
-Lemma inst_subst_to_subst_aux_4 : forall (G : ctx) (tau1 tau2 : ty) (l L : list id)
-                                   (is_s : list ty) (phi : substitution),
+(** This complex lemma is needed to prove [more_general_ctx_disjoint_prefix_apply_inst]. *)
+Lemma inst_subst_to_subst_aux_4 :
+  forall (G : ctx) (tau1 tau2 : ty) (l L : list id)
+    (is_s : list ty) (phi : substitution),
     are_disjoints (FV_ctx G) l ->
     apply_inst_subst is_s (fst (gen_ty_aux tau1 G l)) = Some tau2 ->
     is_prefixe_free2 (FV_ctx G) (snd (gen_ty_aux tau1 G l)) L ->
@@ -667,30 +229,30 @@ Proof.
       fold (apply_subst phi (var i)).
       cases (nth_error is_s i0).
       {  
-         simpl in * |-.
-         inverts* H0.
-         eapply (@image_by_product2 L is_s i i0); eauto.
-         inverts* H1.
-         destruct H0.
-         destruct a.
-         subst.
-         auto. }
+        simpl in * |-.
+        inverts* H0.
+        eapply (@image_by_product2 L is_s i i0); eauto.
+        inverts* H1.
+        destruct H0.
+        destruct a.
+        subst.
+        auto. }
       { inverts* H0. }
-        * rewrite Eq in H0.
-          simpl in H0.
-          cases (nth_error is_s (length l)).
-          { simpl in *.
-            intros.
-            fold (apply_subst phi (var i)).
-            eapply (@image_by_product2 L is_s i (length l)); eauto.
-            inverts* H1.
-            destruct H3.
-            destruct a.
-            subst.
-            apply index_list_id_app; eauto.
-            inverts* H0.
-           }
-          { inverts* H0. }
+      * rewrite Eq in H0.
+        simpl in H0.
+        cases (nth_error is_s (length l)).
+        { simpl in *.
+          intros.
+          fold (apply_subst phi (var i)).
+          eapply (@image_by_product2 L is_s i (length l)); eauto.
+          inverts* H1.
+          destruct H3.
+          destruct a.
+          subst.
+          apply index_list_id_app; eauto.
+          inverts* H0.
+        }
+        { inverts* H0. }
   - crush.
   - intros.
     rewrite fst_gen_aux_arrow_rewrite in H0.
@@ -703,138 +265,65 @@ Proof.
     erewrite (@IHtau1_2 tau3 (snd (gen_ty_aux tau1_1 G l)) L is_s phi); eauto.
     erewrite (@IHtau1_1 tau1 l L is_s phi); eauto.
 Qed.
-    
+
 Hint Resolve inst_subst_to_subst_aux_4.
 Hint Rewrite inst_subst_to_subst_aux_4:RE.
 
-Lemma nth_error_map : forall (s : substitution) (x : list ty) (n : id) (tau : ty),
-    nth_error x n = Some tau ->
-    nth_error (map_extend_subst_type x s) n = Some (apply_subst s tau).
-Proof.
-  induction x; crush.
-  rewrite nth_error_nil in H.
-  inversion H.
-  induction n; crush.
-Qed.
-
-Hint Resolve nth_error_map.
-Hint Rewrite nth_error_map:RE.
-
-Lemma nth_error_k_not_zero : forall a k l, k <> 0 -> nth_error ((var a)::l) k = nth_error l (pred k).
-Proof.
-  induction k; crush.
-Qed.
-
-
-Hint Resolve nth_error_k_not_zero.
-
-Lemma index_list_id_nth : forall (l : list id) (k : id) (i : id),
-    index_list_id i l = Some k -> nth_error (ty_from_id_list l) k = Some (var i).
-Proof.
-  induction l; unfold index_list_id in *. crush.
-  intros.
-  simpl in *. destruct (eq_id_dec a i).
-  inverts* H. subst. reflexivity.
-  erewrite nth_error_k_not_zero.
-  apply IHl.
-  apply index_aux1 in H.
-  auto.
-  destruct k.
-  apply index_aux_false in H; auto. 
-  auto. 
-Qed.
-
-Hint Resolve index_list_id_nth.
-Hint Rewrite index_list_id_nth:RE.
-
-Lemma length_ty_from_id_list : forall l : list id, length (ty_from_id_list l) = length l.
-Proof.
-  induction l; crush.
-Qed.
-
-Hint Resolve length_ty_from_id_list.
-Hint Rewrite length_ty_from_id_list:RE.
-
-Lemma nth_error_app_cons : forall (l : list ty) (tau : ty), nth_error (l ++ tau::nil) (length l) = Some tau.
-simple induction l; auto.
-Qed.
-
-Hint Resolve nth_error_app_cons.
-
-Lemma length_map2 : forall (s : substitution) (l : list id),
-    length (map_extend_subst_type (ty_from_id_list l) s) = length l.
-Proof.
-  simple induction l; auto.
-  intros; simpl in |- *.
-  rewrite H; auto.
-Qed.
-
-Hint Resolve length_map2.
-Hint Rewrite length_map2:RE.
-
-Lemma length_app_cons : forall (A : Set) (l : list A) (x : A), length (l ++ x :: nil) = S (length l).
-Proof.
-  simple induction l; auto.
-  intros; simpl in |- *; auto.
-Qed.
-
-Hint Resolve length_app_cons.
-Hint Rewrite length_app_cons:RE.
-
-Lemma more_general_gen_type_aux : forall (G1 G2 : ctx) (tau1 tau2 : ty) (phi : substitution)
-                                    (l2 l1 L P : list id) (is_s : inst_subst),
+(** This huge lemma is needed to prove [more_general_gen_ty]. *)
+Lemma more_general_ctx_disjoint_prefix_apply_inst :
+  forall (G1 G2 : ctx) (tau1 tau2 : ty) (phi : substitution)
+    (l2 l1 L P : list id) (is_s : inst_subst),
     more_general_ctx G1 G2 -> are_disjoints (FV_ctx G2) l2 ->
     are_disjoints (FV_ctx G1) l1 ->
     apply_inst_subst is_s (fst (gen_ty_aux tau1 G2 l2)) = Some tau2 ->
     is_prefixe_free2 (FV_ctx G2) (snd (gen_ty_aux tau1 G2 l2)) L ->
     product_list L is_s = Some phi ->
     is_prefixe_free2 (FV_ctx G1) (snd (gen_ty_aux tau1 G1 l1)) P ->
-    apply_inst_subst (map_extend_subst_type (ty_from_id_list P) phi)
+    apply_inst_subst (map_apply_subst_over_list_ty (ty_from_id_list P) phi)
                      (fst (gen_ty_aux tau1 G1 l1)) = Some tau2.
 Proof.
- simple induction tau1.
- - do 8 intro; intros more_gen_hyp disjoint1 disjoint2.
-   simpl. 
-   cases (in_list_id i (FV_ctx G1)).
-   erewrite (Sublist.sublist_inv1 i (FV_more_general_ctx more_gen_hyp)); eauto.
-   cases (index_list_id i l1).
-   + simpl.
-     intros.
-     inverts* H2.
-     destruct H3.
-     destruct a.
-     rewrite H2.
-     rewrite (ty_from_id_list_app l1 x).
-     rewrite (map_extend_app phi (ty_from_id_list l1) (ty_from_id_list x)).
-     rewrite (nth_error_app (map_extend_subst_type (ty_from_id_list l1) phi) (map_extend_subst_type (ty_from_id_list x) phi)).
-     erewrite (@nth_error_map phi (ty_from_id_list l1) i0 (var i)).
-     rewrite (@inst_subst_to_subst_aux_4 G2 (var i) tau2 l2 L is_s phi); eauto.
-     eauto.
-     crush.
-   +
-     intros.
-     inverts* H2.
-     destruct H3.
-     destruct a.
-     rename x into P2.
-     simpl in *.
-     rewrite H2.
-     rewrite (ty_from_id_list_app (l1 ++ i::nil) P2).
-     rewrite (map_extend_app phi (ty_from_id_list (l1 ++ i::nil)) (ty_from_id_list P2)).
-     rewrite (nth_error_app (map_extend_subst_type (ty_from_id_list (l1 ++ i::nil)) phi)
-             (map_extend_subst_type (ty_from_id_list P2) phi)).
-     erewrite (@nth_error_map phi (ty_from_id_list (l1 ++ i::nil)) (length l1) (var i)).
-     erewrite (@inst_subst_to_subst_aux_4 G2 (var i) tau2 l2 L is_s phi); eauto.
-     rewrite ty_from_id_list_app; simpl.
-     rewrite <- length_ty_from_id_list; eauto.
-     crush.
+  simple induction tau1.
+  - do 8 intro; intros more_gen_hyp disjoint1 disjoint2.
+    simpl. 
+    cases (in_list_id i (FV_ctx G1)).
+    erewrite (Sublist.sublist_inv1 i (FV_more_general_ctx more_gen_hyp)); eauto.
+    cases (index_list_id i l1).
+    + simpl.
+      intros.
+      inverts* H2.
+      destruct H3.
+      destruct a.
+      rewrite H2.
+      rewrite (ty_from_id_list_app l1 x).
+      rewrite (map_extend_app phi (ty_from_id_list l1) (ty_from_id_list x)).
+      rewrite (nth_error_app (map_apply_subst_over_list_ty
+               (ty_from_id_list l1) phi) (map_apply_subst_over_list_ty (ty_from_id_list x) phi)).
+      erewrite (@nth_error_map phi (ty_from_id_list l1) i0 (var i)).
+      rewrite (@inst_subst_to_subst_aux_4 G2 (var i) tau2 l2 L is_s phi); eauto.
+      eauto.
+      crush.
+    + intros.
+      inverts* H2.
+      destruct H3.
+      destruct a.
+      rename x into P2.
+      simpl in *.
+      rewrite H2.
+      rewrite (ty_from_id_list_app (l1 ++ i::nil) P2).
+      rewrite (map_extend_app phi (ty_from_id_list (l1 ++ i::nil)) (ty_from_id_list P2)).
+      rewrite (nth_error_app (map_apply_subst_over_list_ty (ty_from_id_list (l1 ++ i::nil)) phi)
+                             (map_apply_subst_over_list_ty (ty_from_id_list P2) phi)).
+      erewrite (@nth_error_map phi (ty_from_id_list (l1 ++ i::nil)) (length l1) (var i)).
+      erewrite (@inst_subst_to_subst_aux_4 G2 (var i) tau2 l2 L is_s phi); eauto.
+      rewrite ty_from_id_list_app; simpl.
+      rewrite <- length_ty_from_id_list; eauto.
+      crush.
   - crush. 
-  - 
-    do 11 intro; intros more_gen_hyp disjoint1 disjoint2.
+  - do 11 intro; intros more_gen_hyp disjoint1 disjoint2.
     rewrite fst_gen_aux_arrow_rewrite; intro.
     destruct (@exist_arrow_apply_inst_arrow2  
-              (fst (gen_ty_aux t G2 l2)) (fst (gen_ty_aux t0 G2 (snd (gen_ty_aux t G2 l2))))
-              tau2 is_s H1).
+                (fst (gen_ty_aux t G2 l2)) (fst (gen_ty_aux t0 G2 (snd (gen_ty_aux t G2 l2))))
+                tau2 is_s H1).
     intros.
     destruct H2.
     destructs H2.
@@ -846,76 +335,7 @@ Proof.
     rewrite (@H0 x0 phi (snd (@gen_ty_aux t G2 l2)) (snd (@gen_ty_aux t G1 l1)) L P is_s); eauto.
 Qed.
 
-Hint Resolve more_general_gen_type_aux.
-
-Lemma product_for_le_length : forall (l1 : list id) (l2 : list ty),
-    length l1 <= length l2 -> exists s, product_list l1 l2 = Some s.
-Proof.
-  induction l1; crush.
-  destruct l2; crush. 
-  edestruct IHl1; eauto.
-  apply le_S_n in H.
-  apply H.
-  rewrite H0.
-  exists ((a, t)::x).
-  reflexivity.
-Qed.
-
-Hint Resolve product_for_le_length.
-
-Lemma length_Snd_gen_aux : forall (G : ctx) (tau : ty) (l : list id),
-    length (snd (gen_ty_aux tau G l)) = max (length l) (max_gen_vars (fst (gen_ty_aux tau G l))).
-Proof.
-  induction tau; crush.
-  cases (in_list_id i (FV_ctx G)); crush.
-  rewrite Nat.max_0_r. reflexivity.
-  cases (index_list_id i l).
-  simpl.
-  symmetry.
-  apply max_l.
-  change (i0 < length l) in |- *.
-  eapply index_lt; eauto.
-  simpl.
-  rewrite length_app.
-  simpl.
-  symmetry.
-  assert (S (length l) = length l + 1). auto with *.
-  rewrite H.
-  apply max_r. auto with *.
-  rewrite Nat.max_0_r. reflexivity.
-  cases (gen_ty_aux tau1 G l).
-  cases (gen_ty_aux tau2 G l0).
-  simpl.
-  specialize IHtau1 with (l:=l).
-  rewrite Eq in IHtau1.
-  specialize IHtau2 with (l:=l0).
-  rewrite Eq0 in IHtau2.
-  simpl in *.
-  rewrite IHtau1 in IHtau2.
-  rewrite Nat.max_assoc.
-  assumption.
-Qed.
-
-Lemma product_list_exists : forall (tau : ty) (G : ctx) (is_s : inst_subst),
-    max_gen_vars (gen_ty tau G) <= length is_s ->
-    exists s, product_list (snd (gen_ty_aux tau G nil)) is_s = Some s.
-Proof.
-  intros.
-  apply product_for_le_length.
-  rewrite length_Snd_gen_aux.
-  crush.
-Qed.
-
-
-Lemma is_prefixe_reflexivity : forall C L : list id, is_prefixe_free2 C L L.
-intros C L.
-econstructor.
-exists (nil: list id).
- split; auto.
- apply app_nil_end.
-Qed.
-
-Hint Resolve is_prefixe_reflexivity.
+Hint Resolve more_general_ctx_disjoint_prefix_apply_inst.
 
 Lemma more_general_gen_ty : forall (G1 G2 : ctx) (t : ty),
     more_general_ctx G1 G2 -> more_general (gen_ty t G1) (gen_ty t G2).
@@ -926,23 +346,13 @@ Proof.
   unfold gen_ty in |- *; intros.
   destruct (product_list_exists t G2 x); eauto.
   unfold is_schm_instance.
-  exists (map_extend_subst_type (ty_from_id_list (snd (gen_ty_aux t G1 nil))) x0).
-  rewrite (@more_general_gen_type_aux G1 G2 t tau x0 nil nil
+  exists (map_apply_subst_over_list_ty (ty_from_id_list (snd (gen_ty_aux t G1 nil))) x0).
+  rewrite (@more_general_ctx_disjoint_prefix_apply_inst G1 G2 t tau x0 nil nil
     (snd (gen_ty_aux t G2 nil)) (snd (gen_ty_aux t G1 nil)) x)
  ; eauto.
 Qed.
 
 Hint Resolve more_general_gen_ty.
-
-Lemma has_type_var_ctx_diff : forall (i j : id) (G : ctx) (tau : ty) (sigma : schm),
-    i <> j -> has_type G (var_t i) tau -> has_type ((j, sigma) :: G) (var_t i) tau.
-Proof.
-  intros.
-  inversion_clear H0.
- econstructor; crush.
-Qed.
-
-Hint Resolve has_type_var_ctx_diff.
 
 Lemma typing_in_a_more_general_ctx : forall (e : term) (G2 G1 : ctx) (t : ty),
     more_general_ctx G1 G2 -> has_type G2 e t -> has_type G1 e t.
@@ -994,15 +404,6 @@ Qed.
 
 Hint Resolve more_general_ctx_refl.
 
-Lemma is_not_generalizable_aux : forall (G : ctx) (tau : ty) (l : list id),
-    is_sublist_id (ids_ty tau) (FV_ctx G) ->
-    gen_ty_aux tau G l = (ty_to_schm tau, l).
-Proof.
-  induction tau; crush.
-Qed.
-
-Hint Resolve is_not_generalizable_aux.
-
 Lemma more_general_gen_ty_before_apply_subst_aux : forall (G : ctx) (tau1 tau2 : ty) (phi s : substitution)
                       (l1 l2 L P : list id) (is_s : inst_subst),
     are_disjoints (FV_ctx G) l1 ->
@@ -1011,7 +412,7 @@ Lemma more_general_gen_ty_before_apply_subst_aux : forall (G : ctx) (tau1 tau2 :
     is_prefixe_free2 (FV_ctx (apply_subst_ctx s G)) (snd (gen_ty_aux (apply_subst s tau1) (apply_subst_ctx s G) l2)) L ->
     product_list L is_s = Some phi ->
     is_prefixe_free2 (FV_ctx G) (snd (gen_ty_aux tau1 G l1)) P ->
-    apply_inst_subst (map_extend_subst_type (ty_from_id_list P) (compose_subst s phi))
+    apply_inst_subst (map_apply_subst_over_list_ty (ty_from_id_list P) (compose_subst s phi))
                      (apply_subst_schm s (fst (gen_ty_aux tau1 G l1))) = Some tau2.
 Proof.
   induction tau1.
@@ -1086,7 +487,7 @@ Proof.
   unfold gen_ty in *.
   destruct (product_list_exists (apply_subst s tau) (apply_subst_ctx s G) x); eauto.
   unfold is_schm_instance.
-  exists (map_extend_subst_type (ty_from_id_list (snd (gen_ty_aux tau G nil))) (compose_subst s x0)).
+  exists (map_apply_subst_over_list_ty (ty_from_id_list (snd (gen_ty_aux tau G nil))) (compose_subst s x0)).
   eauto.
 Qed.
 
