src/Nth_error_tools.v
@@ -1,0 +1,58 @@
+Set Implicit Arguments.
+
+Require Import Arith.Arith_base List Omega.
+Require Import Wellfounded.Lexicographic_Product.
+Require Import Relation_Operators.
+Require Import Coq.Setoids.Setoid.
+Require Import Program.
+Require Import SimpleTypes.
+Require Import Subst.
+Require Import LibTactics.
+Require Import MyLtacs.
+
+
+Lemma nth_error_nil : forall i, nth_error (nil : list ty) i = None.
+Proof.
+  intros.
+  induction i; mysimp.
+Qed.
+
+Hint Resolve nth_error_nil.
+Hint Rewrite nth_error_nil:RE.
+
+Lemma nth_error_map : forall (s : substitution) (x : list ty) (n : id) (tau : ty),
+    nth_error x n = Some tau ->
+    nth_error (map_apply_subst_over_list_ty x s) n = Some (apply_subst s tau).
+Proof.
+  induction x; crush.
+  rewrite nth_error_nil in H.
+  inversion H.
+  induction n; crush.
+Qed.
+
+Hint Resolve nth_error_map.
+Hint Rewrite nth_error_map:RE.
+
+Lemma nth_error_k_not_zero : forall a k l, k <> 0 -> nth_error ((var a)::l) k = nth_error l (pred k).
+Proof.
+  induction k; crush.
+Qed.
+
+Hint Resolve nth_error_k_not_zero.
+
+Lemma nth_error_app_cons : forall (l : list ty) (tau : ty), nth_error (l ++ tau::nil) (length l) = Some tau.
+simple induction l; auto.
+Qed.
+
+Hint Resolve nth_error_app_cons.
+
+Lemma nth_error_app : forall (l l1 : list ty) (n : id), n < length l -> nth_error (l ++ l1) n = nth_error l n.
+Proof.
+  induction l; crush.
+  induction n; crush.
+  erewrite <- IHl; crush.
+Qed.
+
+Hint Resolve nth_error_app.
+Hint Rewrite nth_error_app:RE.
+
