src/Product_list.v
@@ -1,0 +1,105 @@
+Set Implicit Arguments.
+
+Require Import List.
+Require Import Sublist.
+Require Import ListIds.
+Require Import Context.
+Require Import Typing.
+Require Import Gen.
+Require Import SimpleTypes.
+Require Import Schemes.
+Require Import Subst.
+Require Import SubstSchm.
+Require Import MyLtacs.
+Require Import Nth_error_tools.
+Require Import LibTactics.
+
+
+Fixpoint product_list (l1 : list id) (l2 : list ty) :=
+  match l1 with
+  | nil =>  Some nil
+  | st :: l'1 => match l2 with
+                | nil => None
+                | t :: l'2 => match product_list l'1 l'2 with
+                             | None => None
+                             | Some s => Some ((st, t) :: s)
+                             end
+                end
+  end.
+
+Lemma domain_product : forall (l : list id) (is_s : inst_subst) (phi : substitution),
+    product_list l is_s = Some phi -> dom phi = l.
+Proof.
+  induction l. crush.
+  destruct is_s. crush.
+  intros. 
+  simpl in *.
+  cases (product_list l is_s).
+  inverts* H.
+  simpl.
+  erewrite IHl; eauto.
+  inverts* H.
+Qed.  
+
+Lemma image_by_product2 : forall (l : list id) (is_s : inst_subst) (st : id) 
+                            (n0 : id) (phi : substitution) (tau : ty),
+    index_list_id st l = Some n0 ->
+    product_list l is_s = Some phi ->
+    nth_error is_s n0 = Some tau -> apply_subst phi (var st) = tau.
+Proof.
+  induction l; unfold index_list_id. crush.
+  intros.
+  simpl in *.
+  destruct (eq_id_dec a st).
+  inverts* H.
+  destruct is_s.
+  inversion H0.
+  subst.
+  simpl in H1. inverts* H1.
+  cases (product_list l is_s).
+  inverts* H0.
+  crush.
+  inversion H0.
+  destruct is_s.
+  inversion H0.
+  cases (product_list l is_s).
+  inverts* H0.
+  crush.
+  eapply IHl.
+  apply index_aux1 in H.
+  unfold index_list_id. apply H.
+  apply Eq.
+  destruct n0. simpl in *.
+  inverts* H1. destruct is_s.
+  assert (False). { eapply index_aux_false with (n := 1) (m := 0); eauto. } contradiction.
+  assert (False). { eapply index_aux_false with (n := 1) (m := 0); eauto. } contradiction.
+  simpl. eauto.
+  inversion H0.
+Qed.
+
+Hint Resolve image_by_product2.
+
+Lemma product_for_le_length : forall (l1 : list id) (l2 : list ty),
+    length l1 <= length l2 -> exists s, product_list l1 l2 = Some s.
+Proof.
+  induction l1; crush.
+  destruct l2; crush. 
+  edestruct IHl1; eauto.
+  apply le_S_n in H.
+  apply H.
+  rewrite H0.
+  exists ((a, t)::x).
+  reflexivity.
+Qed.
+
+Hint Resolve product_for_le_length.
+
+Lemma product_list_exists : forall (tau : ty) (G : ctx) (is_s : inst_subst),
+    max_gen_vars (gen_ty tau G) <= length is_s ->
+    exists s, product_list (snd (gen_ty_aux tau G nil)) is_s = Some s.
+Proof.
+  intros.
+  apply product_for_le_length.
+  rewrite length_Snd_gen_aux.
+  crush.
+Qed.
